coq/ZF/Meta/Test/Class/Incl.v
@@ -2,51 +2,21 @@ Require Import Coq.Lists.List.
 Require Import Coq.Strings.String.
 
 Require Import ZF.Meta.Ctx.
-Require Import ZF.Meta.Decl.
 Require Import ZF.Meta.Env.
-Require Import ZF.Meta.HasTyDecl.
 Require Import ZF.Meta.HasTy.
 Require Import ZF.Meta.HasTyIn.
 Require Import ZF.Meta.Term.
 Require Import ZF.Meta.Ty.
 
+Require Import ZF.Meta.Test.Decl.Class.Equiv.
+Require Import ZF.Meta.Test.Decl.Class.Incl.
+
 Import ListNotations.
-
-(* Declarations.                                                                *)
-
-(* Definition toClass (a:U) : Class := fun x => x :< a.                         *)
-Definition toClass : Decl :=
-  {| para := [TySet];
-     res  := TyClass;
-     body := Some (Lam (Elem (Var 0) (Var 1))) |}.
-
-(* Definition equiv (P Q:Class) : Prop := forall x, P x <-> Q x.                *)
-Definition equiv : Decl :=
-  {| para := [TyClass; TyClass];
-     res  := TyProp;
-     body := Some
-       (All VarTySet
-         (Iff
-           (App (Var 2) (Var 0))
-           (App (Var 1) (Var 0)))) |}.
-
-(* Definition Incl (P Q:Class) : Prop := forall x, P x -> Q x.                  *)
-Definition Incl : Decl :=
-  {| para := [TyClass; TyClass];
-     res  := TyProp;
-     body := Some
-       (All VarTySet
-         (Imp
-           (App (Var 2) (Var 0))
-           (App (Var 1) (Var 0)))) |}.
 
 (* Environment.                                                                 *)
 
-Definition env : Env := fun name =>
-  if String.eqb name "toClass" then Some toClass else
-  if String.eqb name "equiv"   then Some equiv else
-  if String.eqb name "Incl"    then Some Incl else
-  None.
+Definition env : Env := Env.unions
+  [ZF.Meta.Test.Decl.Class.Incl.env; ZF.Meta.Test.Decl.Class.Equiv.env].
 
 (* Propositions.                                                                *)
 
@@ -125,171 +95,50 @@ Definition Tran : Term :=
             (Ident "Incl" [Var 1; Var 0])
             (Ident "Incl" [Var 2; Var 0]))))).
 
-(* Declaration typing.                                                          *)
-
-(* The declaration body for toClass maps a set to its membership class.         *)
-Proposition toClassHasTyDecl : HasTyDecl Env.empty toClass.
-Proof.
-  (* Proof by Hermes + gpt 5.5                                                  *)
-  apply HasTyLam, HasTyElem; apply (HasTyVar _ _ _ TySet); reflexivity.
-Qed.
-
-(* The declaration body for equivalence compares two classes pointwise.         *)
-Proposition equivHasTyDecl : HasTyDecl Env.empty equiv.
-Proof.
-  (* Proof by Hermes + gpt 5.5                                                  *)
-  apply HasTyAll, HasTyIff.
-  - apply HasTyApp.
-    + apply (HasTyVar _ _ _ TyClass). reflexivity.
-    + apply (HasTyVar _ _ _ TySet). reflexivity.
-  - apply HasTyApp.
-    + apply (HasTyVar _ _ _ TyClass). reflexivity.
-    + apply (HasTyVar _ _ _ TySet). reflexivity.
-Qed.
-
-(* The declaration body for inclusion compares two classes pointwise.           *)
-Proposition InclHasTyDecl : HasTyDecl Env.empty Incl.
-Proof.
-  (* Proof by Hermes + gpt 5.5                                                  *)
-  apply HasTyAll, HasTyImp.
-  - apply HasTyApp.
-    + apply (HasTyVar _ _ _ TyClass). reflexivity.
-    + apply (HasTyVar _ _ _ TySet). reflexivity.
-  - apply HasTyApp.
-    + apply (HasTyVar _ _ _ TyClass). reflexivity.
-    + apply (HasTyVar _ _ _ TySet). reflexivity.
-Qed.
-
-(* Identifier typing.                                                           *)
-
-(* The identifier toClass sends a set argument to a class.                      *)
-Proposition toClassHasTy :
-  HasTyIn env [TySet] (Ident "toClass" [Var 0]) TyClass.
-Proof.
-  (* Proof by Hermes + gpt 5.5                                                  *)
-  apply HasTyIdent with (argTys := [TySet]). 1: reflexivity.
-  apply HasTysCons.
-  - apply (HasTyVar _ _ _ TySet). reflexivity.
-  - apply HasTysNil.
-Qed.
-
-(* The identifier toClass sends any set variable to a class.                    *)
-Proposition toClassVarHasTy : forall (G:Ctx) (n:nat),
-  typeOf G n = Some TySet ->
-  HasTyIn env G (Ident "toClass" [Var n]) TyClass.
-Proof.
-  (* Proof by Hermes + gpt 5.5                                                  *)
-  intros G n H1.
-  apply HasTyIdent with (argTys := [TySet]). 1: reflexivity.
-  apply HasTysCons.
-  - apply HasTyVar. assumption.
-  - apply HasTysNil.
-Qed.
-
-(* The identifier equiv sends two class arguments to a proposition.             *)
-Proposition equivHasTy :
-  HasTyIn env [TyClass; TyClass]
-    (Ident "equiv" [Var 1; Var 0]) TyProp.
-Proof.
-  (* Proof by Hermes + gpt 5.5                                                  *)
-  apply HasTyIdent with (argTys := [TyClass; TyClass]). 1: reflexivity.
-  apply HasTysCons.
-  - apply (HasTyVar _ _ _ TyClass). reflexivity.
-  - apply HasTysCons.
-    + apply (HasTyVar _ _ _ TyClass). reflexivity.
-    + apply HasTysNil.
-Qed.
-
-(* Equivalence applied to two class variables is well sorted.                   *)
-Proposition equivVarsHasTy : forall (G:Ctx) (m n:nat),
-  typeOf G m = Some TyClass ->
-  typeOf G n = Some TyClass ->
-  HasTyIn env G (Ident "equiv" [Var m; Var n]) TyProp.
-Proof.
-  (* Proof by Hermes + gpt 5.5                                                  *)
-  intros G m n H1 H2.
-  apply HasTyIdent with (argTys := [TyClass; TyClass]). 1: reflexivity.
-  apply HasTysCons.
-  - apply HasTyVar. assumption.
-  - apply HasTysCons.
-    + apply HasTyVar. assumption.
-    + apply HasTysNil.
-Qed.
-
-(* The identifier Incl sends two class arguments to a proposition.              *)
-Proposition InclHasTy :
-  HasTyIn env [TyClass; TyClass]
-    (Ident "Incl" [Var 1; Var 0]) TyProp.
-Proof.
-  (* Proof by Hermes + gpt 5.5                                                  *)
-  apply HasTyIdent with (argTys := [TyClass; TyClass]). 1: reflexivity.
-  apply HasTysCons.
-  - apply (HasTyVar _ _ _ TyClass). reflexivity.
-  - apply HasTysCons.
-    + apply (HasTyVar _ _ _ TyClass). reflexivity.
-    + apply HasTysNil.
-Qed.
-
-(* Inclusion applied to two class variables is well sorted.                     *)
-Proposition InclVarsHasTy : forall (G:Ctx) (m n:nat),
-  typeOf G m = Some TyClass ->
-  typeOf G n = Some TyClass ->
-  HasTyIn env G (Ident "Incl" [Var m; Var n]) TyProp.
-Proof.
-  (* Proof by Hermes + gpt 5.5                                                  *)
-  intros G m n H1 H2.
-  apply HasTyIdent with (argTys := [TyClass; TyClass]). 1: reflexivity.
-  apply HasTysCons.
-  - apply HasTyVar. assumption.
-  - apply HasTysCons.
-    + apply HasTyVar. assumption.
-    + apply HasTysNil.
-Qed.
-
 (* Proposition typing.                                                          *)
 
 (* Double inclusion and equivalence form a well-sorted proposition.             *)
-Proposition DoubleHasTy : HasTyIn env Ctx.empty Double TyProp.
+Proposition DoubleCheck : HasTyIn env Ctx.empty Double TyProp.
 Proof.
   (* Proof by Hermes + gpt 5.5                                                  *)
   apply HasTyAll, HasTyAll, HasTyIff.
-  - apply equivVarsHasTy; reflexivity.
-  - apply HasTyAnd; apply InclVarsHasTy; reflexivity.
+  - apply equivCheckIdent; reflexivity.
+  - apply HasTyAnd; apply InclCheckIdent; reflexivity.
 Qed.
 
 (* Compatibility of inclusion with equivalence is well sorted.                  *)
-Proposition EquivCompatHasTy : HasTyIn env Ctx.empty EquivCompat TyProp.
+Proposition EquivCompatCheck : HasTyIn env Ctx.empty EquivCompat TyProp.
 Proof.
   (* Proof by Hermes + gpt 5.5                                                  *)
   apply HasTyAll, HasTyAll, HasTyAll, HasTyAll, HasTyImp.
-  - apply equivVarsHasTy; reflexivity.
+  - apply equivCheckIdent; reflexivity.
   - apply HasTyImp.
-    + apply equivVarsHasTy; reflexivity.
+    + apply equivCheckIdent; reflexivity.
     + apply HasTyImp.
-      * apply InclVarsHasTy; reflexivity.
-      * apply InclVarsHasTy; reflexivity.
+      * apply InclCheckIdent; reflexivity.
+      * apply InclCheckIdent; reflexivity.
 Qed.
 
 (* Left compatibility of inclusion with equivalence is well sorted.             *)
-Proposition EquivCompatLHasTy : HasTyIn env Ctx.empty EquivCompatL TyProp.
+Proposition EquivCompatLCheck : HasTyIn env Ctx.empty EquivCompatL TyProp.
 Proof.
   (* Proof by Hermes + gpt 5.5                                                  *)
   apply HasTyAll, HasTyAll, HasTyAll, HasTyImp.
-  - apply equivVarsHasTy; reflexivity.
-  - apply HasTyImp; apply InclVarsHasTy; reflexivity.
+  - apply equivCheckIdent; reflexivity.
+  - apply HasTyImp; apply InclCheckIdent; reflexivity.
 Qed.
 
 (* Right compatibility of inclusion with equivalence is well sorted.            *)
-Proposition EquivCompatRHasTy : HasTyIn env Ctx.empty EquivCompatR TyProp.
+Proposition EquivCompatRCheck : HasTyIn env Ctx.empty EquivCompatR TyProp.
 Proof.
   (* Proof by Hermes + gpt 5.5                                                  *)
   apply HasTyAll, HasTyAll, HasTyAll, HasTyImp.
-  - apply equivVarsHasTy; reflexivity.
-  - apply HasTyImp; apply InclVarsHasTy; reflexivity.
+  - apply equivCheckIdent; reflexivity.
+  - apply HasTyImp; apply InclCheckIdent; reflexivity.
 Qed.
 
 (* Reflexivity of inclusion is a well-sorted proposition.                       *)
-Proposition ReflHasTy : HasTyIn env Ctx.empty Refl TyProp.
+Proposition ReflCheck : HasTyIn env Ctx.empty Refl TyProp.
 Proof.
   (* Proof by Hermes + gpt 5.5                                                  *)
   apply HasTyAll.
@@ -302,21 +151,21 @@ Proof.
 Qed.
 
 (* Antisymmetry of inclusion is a well-sorted proposition.                      *)
-Proposition AntiHasTy : HasTyIn env Ctx.empty Anti TyProp.
+Proposition AntiCheck : HasTyIn env Ctx.empty Anti TyProp.
 Proof.
   (* Proof by Hermes + gpt 5.5                                                  *)
   apply HasTyAll, HasTyAll, HasTyImp.
-  - apply InclVarsHasTy; reflexivity.
+  - apply InclCheckIdent; reflexivity.
   - apply HasTyImp.
-    + apply InclVarsHasTy; reflexivity.
-    + apply equivVarsHasTy; reflexivity.
+    + apply InclCheckIdent; reflexivity.
+    + apply equivCheckIdent; reflexivity.
 Qed.
 
 (* Transitivity of inclusion is a well-sorted proposition.                      *)
-Proposition TranHasTy : HasTyIn env Ctx.empty Tran TyProp.
+Proposition TranCheck : HasTyIn env Ctx.empty Tran TyProp.
 Proof.
   (* Proof by Hermes + gpt 5.5                                                  *)
   apply HasTyAll, HasTyAll, HasTyAll, HasTyImp.
-  - apply InclVarsHasTy; reflexivity.
-  - apply HasTyImp; apply InclVarsHasTy; reflexivity.
+  - apply InclCheckIdent; reflexivity.
+  - apply HasTyImp; apply InclCheckIdent; reflexivity.
 Qed.
